Composition/Protocol.v
@@ -7,13 +7,15 @@ From Bythos.Composition Require Export Types.
 From RecordUpdate Require Import RecordUpdate.
 
 (* Seq: Pt1 --> Pt2, unidirection *)
-
+(* since the two protocols will run in the same environment, make their BTh the same *)
 Module Type SeqCompProtocolTrigger (A : NetAddr) (M1 M2 : MessageType) (BTh : ByzThreshold A)
   (Pk1 : SimplePacket A M1) (Pk2 : SimplePacket A M2)
   (Pt1 : Protocol.Protocol A M1 Pk1 BTh)
   (Pt2 : Protocol.Protocol A M2 Pk2 BTh).
 
-Parameter trigger_procMsg : Pt1.State -> Pt1.State -> option Pt2.InternalTransition.
+(* trigger: check whether Pt2.procInt should be triggered after Pt1.procInt/Pt1.procMsg, 
+    based on the change of the local state for Pt1 *)
+Parameter trigger_procMsg : Pt1.State (* old local state *) -> Pt1.State (* new local state *) -> option Pt2.InternalTransition.
 Parameter trigger_procInt : Pt1.State -> Pt1.State -> option Pt2.InternalTransition.
 
 End SeqCompProtocolTrigger.
@@ -71,16 +73,3 @@ Definition procMsg st src msg :=
   end.
 
 End SeqCompProtocol.
-(*
-Module SeqCompProtocolImpl (Export A : NetAddr) (M1 M2 : MessageType) (BTh : ByzThreshold A)
-  (CM : CompMessage M1 M2) (Pk1 : SimplePacket A M1) (Pk2 : SimplePacket A M2)
-  (CPk : CompSimplePacket A M1 M2 CM Pk1 Pk2)
-  (Pt1 : Protocol.Protocol A M1 Pk1 BTh)
-  (Pt2 : Protocol.Protocol A M2 Pk2 BTh) 
-  (SCPT : SeqCompProtocolTrigger A M1 M2 BTh Pk1 Pk2 Pt1 Pt2)
-  <: Protocol.Protocol A CM CPk BTh <: SeqCompProtocol A M1 M2 BTh CM Pk1 Pk2 CPk Pt1 Pt2 SCPT.
-
-Include SeqCompProtocol A M1 M2 BTh CM Pk1 Pk2 CPk Pt1 Pt2 SCPT.
-
-End SeqCompProtocolImpl.
-*)
